\documentclass{article}

\usepackage[bmargin=0.25in]{geometry}
\usepackage{amsmath, amssymb, amsthm}
\usepackage{listings}
\usepackage{multicol}
\usepackage{enumerate,enumitem}

\title{CSCI 305 HW 8}
\author{Isaac Boaz}

\begin{document}
\maketitle

Use the loop invariant `at step \(i, k = \sum_{m=1}^{i}{2^m}\) after line 6 evaluates' to show that the code is a correct algorithm to compute \(\sum_{m=1}^{n}{2^m}\).

\begin{proof}
      By Induction. \\
      \textbf{Base Case} \(n = 1\) \\
      We observe that the given code returns 2 which is \(= \sum_{m=1}^{2} 2^m\). \\[1em]
      \textbf{Inductive Step} Suppose \(k_{i-1} = \sum_{m=1}^{i-1}{2^m}\). Then
      \begin{align*}
            k_{i} & = k_{i-1} + \ell(i)           \\
                  & = \sum_{m=1}^{i-1}{2^m} + 2^i \\
                  & = \sum_{m=1}^{i}{2^m}
      \end{align*}
      \textbf{Conclusion} By induction, the code is a correct algorithm to compute \(\sum_{m=1}^{n}{2^m}\) where \(i = n\).
\end{proof}

\end{document}